#+title: Lösungen zum 6. Übungsblatt
#+date: 2017-05-16
#+email: tobias.denkinger@tu-dresden.de
#+options: toc:nil

* Lösung zu Aufgabe 12.4.29

#+begin_src lisp
; (a)  A t s u ⇒* s
A = (λxyz. y)

; (b)  B t s ⇒* s t
B = (λxy. yx)

; (c)  C C ⇒ᵦ C C
;      (λx. xx) (λx. xx) ⇒ᵦ (λx. xx) (λx. xx)
C = (λx. xx)

; (d)  D ⇒ᵦ D
D = C C

; (e)  E E t ⇒* E t E
E = (λxy. xyx)
#+end_src


* Lösung zu Aufgabe 12.4.32

#+begin_src lisp
; (a)
   (λfx. ffx)(λy. x)z
      ------ -------
      GV={x} FV={x}

⇒ₐ (λfx₁. ffx₁)(λy. x)z      ; ⇒ₐ steht für α-Konversion 

⇒ᵦ  (λx₁. (λy. x)(λy. x)x₁) z   
          ---------------- --
          GV={y}           FV={z}

⇒ᵦ  (λy. x)(λy. x)z
        -- ------
      GV=∅ FV={x}

⇒ᵦ  xz

; (b)
; ⟨Y⟩ = (λh. (λy. h(yy))(λy. h(yy)))
⟨Y⟩⟨F⟩
=  (λh. (λy. h(yy))(λy. h(yy)))⟨F⟩
⇒* (λy.⟨F⟩(yy))(λy. ⟨F⟩(yy)) = ⟨t_F⟩ ⟨t_F⟩
⇒* ⟨F⟩ ((λy. ⟨F⟩(yy))(λy. ⟨F⟩(yy))) = ⟨F⟩ (⟨t_F⟩ ⟨t_F⟩)

⟨Y⟩⟨F⟩⟨6⟩⟨5⟩⟨3⟩

⇒* ⟨F⟩ (⟨t_F⟩ ⟨t_F⟩) ⟨6⟩ ⟨5⟩ ⟨3⟩

⇒* ⟨ite⟩ (⟨iszero⟩ (⟨sub⟩ ⟨6⟩ ⟨5⟩)) (…) (⟨succ⟩ ((⟨t_F⟩ ⟨t_F⟩) (⟨pred⟩⟨6⟩) (⟨succ⟩⟨5⟩) (⟨mult⟩⟨2⟩⟨3⟩)))
         --------------------------                            ----------- ----------- --------------
         ⇒* ⟨false⟩                                            ⇒* ⟨5⟩      ⇒* ⟨6⟩      ⇒* ⟨6⟩

⇒* ⟨succ⟩ ((⟨t_F⟩ ⟨t_F⟩) ⟨5⟩ ⟨6⟩ ⟨6⟩) -- optional

⇒* ⟨succ⟩ (⟨F⟩ (⟨t_F⟩ ⟨t_F⟩) ⟨5⟩ ⟨6⟩ ⟨6⟩)

⇒* ⟨succ⟩ (⟨ite⟩ (⟨iszero⟩ (⟨sub⟩⟨5⟩⟨6⟩)) (⟨add⟩⟨6⟩⟨6⟩) (…))
                 ------------------------ -------------
                 ⇒* ⟨true⟩                ⇒* ⟨12⟩

⇒* ⟨succ⟩⟨12⟩ ⇒* ⟨13⟩

; (c)  g = ⟨Y⟩⟨G⟩
⟨G⟩ = λgxy. ⟨ite⟩ (⟨iszero⟩x)
                  (⟨mult⟩⟨2⟩(⟨succ⟩y))
                  (⟨ite⟩ (⟨iszero⟩y)
                         (⟨mult⟩⟨2⟩(⟨succ⟩x))
                         (⟨add⟩⟨4⟩(g(⟨pred⟩x)(⟨pred⟩y)))
                  )
#+end_src


* Lösung zu Aufgabe 12.4.30

#+begin_src lisp
; (a)  Hausaufgabe
(λfx. f(fx))(λy. x)y

; (b)  g = ⟨Y⟩⟨G⟩
⟨G⟩ = λgmn. ⟨ite⟩ (⟨iszero⟩n)
                  m
                  (⟨ite⟩ (⟨iszero⟩(⟨pred⟩n))
                         (⟨succ⟩m)
                         (⟨add⟩(g m (⟨sub⟩n⟨2⟩))(g m (⟨pred⟩n)))
                  )

; (c)
⟨Y⟩⟨F⟩
=  (λh. (λy. h(yy))(λy. h(yy)))⟨F⟩
⇒* (λy.⟨F⟩(yy))(λy. ⟨F⟩(yy)) = ⟨Y_F⟩
⇒* ⟨F⟩ ((λy. ⟨F⟩(yy))(λy. ⟨F⟩(yy))) = ⟨F⟩ ⟨Y_F⟩

⟨Y⟩⟨F⟩⟨2⟩⟨1⟩

⇒* ⟨F⟩ ⟨Y_F⟩ ⟨2⟩ ⟨1⟩

⇒* ⟨ite⟩ (⟨iszero⟩⟨1⟩) (…) (⟨mult⟩⟨2⟩(⟨Y_F⟩⟨2⟩(⟨pred⟩⟨1⟩)))
         -------------                        -----------
         ⇒* ⟨false⟩                           ⇒* ⟨0⟩

⇒* ⟨mult⟩ ⟨2⟩ (⟨Y_F⟩⟨2⟩⟨0⟩)

⇒* ⟨mult⟩ ⟨2⟩ (⟨F⟩⟨Y_F⟩⟨2⟩⟨0⟩)

⇒* ⟨mult⟩ ⟨2⟩ (⟨ite⟩ (⟨iszero⟩⟨0⟩) ⟨1⟩ (…))
                     -------------
                     ⇒* ⟨true⟩

⇒* ⟨mult⟩ ⟨2⟩ ⟨1⟩

⇒* ⟨2⟩
#+end_src
